---
aliases: [Multiplying Plolynomials]
tags: [CSCI532, algorithm, algs]
projects: [Advanced Algorithms]
title: Multiplying Polynomials
linter-yaml-title-alias: Multiplying Polynomials
date created: Tuesday, January 24th 2023, 8:49:10 am
date modified: Friday, January 27th 2023, 11:40:35 am
---

# Multiplying Polynomials

## Naive Approach

input:  
	$A(x) = a_0 + a_1 x + a_2 x^2 + \cdots +a_{n-1}x^{n-1}$  
	$B(x) = b_0 + b_1 x + b_2 x^2 + \cdots +b_{n-1}x^{n-1}$  
Output:  
	$C(x) = A(x) \times B(x) = c_0 + c_1 x + c_2 x^2 + \cdots +c_{2(n-1)}x^{2(n-1)}$

$\underbrace{x_k = \sum_{i=0}^k a_i*b_{(k-i)}}_{O(n)}$  
Using this to calculate $C(x)$ with above takes $O(n^2)$

## Divide and Conquer

Same input as the [[#Naive Approach]]  
Split  
	$$\begin{align}  
	A(x) & = \left[a_0 + a_1 x + \cdots a_{\frac{n}{2} - 1}x^{\frac{n}{2}-1}\right] + \left[a_{\frac{n}{2}}x^{\frac{n}{2}} + \cdots a_{n-1}x^{n-1}\right]\\  
	& = \underbrace{\left[a_0 + a_1 x + \cdots a_{\frac{n}{2} - 1}x^{\frac{n}{2}-1}\right]}_{A_0(x)} + x^{\frac{n}{2}}\underbrace{\left[a_{\frac{n}{2}} + a_{\frac{n}{2}+1}x + \cdots a_{n-1}x^{\frac{n}{2}-1}\right]}_{A_1(x)}a  
	\end{align}$$	Similarly: $$ B(x)= B_0(x)+B_1(x)$$
Then: $$
\begin{align}A(x)\times B(x) & = \left[A_0(x)+ x^{\frac{n}{2}}A_1(x)\right]\left[B_0(x)+x^{\frac{n}{2}}B_1(x)\right]\\ &= A_0(x)\times B_0(x) + x^{\frac{n}{2}}\underbrace{\left[A_0(x)\times B_1(x) + A_1(x)\times B_0(x)\right]}_\phi + x^nA_1(x)B_1(x)\end{align}
$$$$\phi = \left[\left\{A_0(x)+A_1(x)\right\}\times \left\{B_0(x)+B_1(x)\right\}\right] - \left[A_0(x)\times B_0(x) + A_1(x)\times B_1(x)\right]$$

Recurrence Relation  
$T(n) = 3 \cdot T(n/2) + f(n)$ s.t. $f(n) \in O(n)$

Using the Master Theorem of Recurrences, [[202301241003]], since $f(n)\in O(n) \subset O(n^{\log_2 3})$ (in the phrasing of the Master Theorem for Recurrences this would give $\epsilon \approx 0.58$) $\rightarrow T(n)\in \Theta\left(n^{\log_23}\right) \approx \Theta \left(n^{1.58}\right)$. This is obviously better than $O(n^2)$ from the naive approach.  

## FFT
$A(x)\times B(x)=C(x)$, $C(x)$ will be a polynomial with at most $2n-1$ terms, where $n$ is the larger degree of $A(x)$ and $B(x)$. So, we know that we need at least $2n-1 \rightarrow 2n$. Using Hormer’s Rule, this problem is $O(n^2)$.

$A, B$: Function form $\rightarrow$ Point form - DFT  
$A(x)\times B(x) = C(x)$: in Point form - Hormer’s Rule $O(n)$  
$C(x)$: Point form $\rightarrow$ Function form - DFT$^{-1}$

This altogether takes $O(n \cdot \lg n)$  

### DFT:
$y_k = A\left(\omega_n^k\right)$
$\vec{y} = \text{DFT}_n\left(\vec{a}\right)$
$A(x)= A^{[0]}\left(x^2\right)+x\cdot A^{[1]}\left(x^2\right)$ $\longleftarrow$ This is our recursive setup

RECURSIVE-DFT$(a)$:
	let $n = \text{length(a)}$ 
	if $n = 1$ 
		return $a$
	$\omega_n = e^{i \frac{2\pi}{n}}$
	$w = 1$                (current root)
	$a^{[0]} = \left(a_0, a_2, a_4, \cdots , a_{n-2}\right)$
	$a^{[1]} = \left(a_1, a_3, a_5, \cdots, a_{n-1}\right)$
	$y^{[0]} =$ RECURSIVE-DFT$\left(a^{[0]}\right)$
	$y^{[1]} =$ RECURSIVE-DFT$\left(a^{[1]}\right)$
	for $k = 0$ to $\frac{n}{2}-1$ {[^1]
		$y_k = y_k^{[0]} + w \cdot y_k^{[1]}$[^2]
		$y_{y + n/2} = y_k^{[0]} - w \cdot y_k^{[1]}$
		$w = w\cdot \omega_n$
	}
	return $y$ 

$T(n) = 2\cdot T(n/2)+O(n) \in \Theta\left(n\cdot\lg n\right) = \tilde{\Theta} (n)$ 

### DFT$^{-1}$ 
$$y_k = \sum_{j=0}^{n-1} a_j \left(\omega_n^k\right)^j$$
or $$\vec{y}= V_n \cdot \vec{a}$$
s.t. $$V_n = \begin{bmatrix}1 & 1& 1 & \cdots & 1 \\ 1 & \omega_n & \omega_n^2 & \cdots &\omega_n^{n-1}\\ 1 & \left(\omega_n^2\right) & \left(\omega_n^2\right)^2 &\cdots &\left(\omega_n^2\right)^{n-1} \\ \vdots & \vdots & \vdots & \ddots & \vdots\\ 1 & \left(\omega_n^{n-1}\right) & \left(\omega_n^{n-1}\right)^2 & \cdots & \left(\omega_n^{n-1}\right)^{n-1}\end{bmatrix}$$ and thus $$\left[V_n^{-1}\right]_{jk} = \frac{1}{n} \; \omega_n^{-j\cdot k}\; ,$$$$\vec{a} = V^{-1}\cdot \vec{y} \; \longrightarrow \; a_j = \frac{1}{n}\, \sum_{k=0}^{n-1} \,y_k \; \left(\omega_n^{-k}\right)^{j} \; .$$This gives RECURSIVE-DFT s.t. 
- switch $a_k \longleftrightarrow y_k$ 
- replace $\omega_n$ with $\omega_n^{-1}$
- divide $a_k$’s by $n$

[^1]: 
[^2]: 